StateT monad transformer, InjL, InjR, Case.
Added a StateT monad transformer for state, in order to have better
notation than working with (val * state). Added interpreter cases for
InjL, InjR, and Case.

src/go_lang/interpreter.v
@@ -16,8 +16,8 @@ Delimit Scope val_scope with V.
 
 Section go_lang_int.
   Context {ext: ext_op} {ffi: ffi_model}
-          {ffi_semantics: ext_semantics ext ffi}.
-          {ffi_interprable: ext_interprable ext ffi}.
+          {ffi_semantics: ext_semantics ext ffi}
+          {ffi_interpretable: @ext_interpretable ext ffi}.
   Canonical Structure heap_ectxi_lang := (EctxiLanguage (heap_lang.heap_lang_mixin ffi_semantics)).
   Canonical Structure heap_ectx_lang := (EctxLanguageOfEctxi heap_ectxi_lang).
   Canonical Structure heap_lang := (LanguageOfEctx heap_ectx_lang).
@@ -26,82 +26,162 @@ Section go_lang_int.
 Notation "x <- p1 ; p2" := (mbind (fun x => p2) p1) 
                               (at level 60, right associativity).
 
-Fixpoint interpret (e: expr) (fuel: nat) : option val :=  
+(* http://hackage.haskell.org/package/mtl-2.2.2/docs/Control-Monad-State-Lazy.html#t:StateT *)
+(* This is a state monad transformer, which takes a pre-existing monad M and produces a new monad StateT M. *)
+Inductive StateT M (X: Type) : Type :=
+| StateFn (f : (state -> M (prod X state)))
+.
+
+(* Turns a StateT M X back into a function (input state) -> M (X, ending state) *)
+Definition runStateT {M} {X: Type} (mf: StateT M X) (s: state) : M (prod X state) :=
+  match mf with
+  | StateFn _ _ f => f s
+  end.
+
+(* fmap, join, bind, and ret definitions for the monad StateT M,
+ * defined in terms of the corresponding monad operations for the monad M. *)
+Definition StateT_fmap M (mf : FMap M) : FMap (StateT M) :=
+  (fun A B f => (fun sa => match sa with
+                 | StateFn _ _ sf =>
+                   StateFn _ _ (fun s => (mf _ _ (fun p => match p with
+                                             | (x, s') => (f x, s')
+                                             end))(sf s))
+                 end)).
+
+Definition StateT_join M (mf : FMap M) (mj : MJoin M) : MJoin (StateT M) :=
+  (fun A ssm => match ssm with
+             | StateFn _ _ ssf =>
+               StateFn _ _ (fun st =>
+                              mjoin ((fun (p : (StateT M A * state)%type) =>
+                                        match p with
+                                        | (StateFn _ _ sf, st') => (sf st')
+                                        end) <$> (ssf st)))
+             end).
+
+Definition StateT_bind M (mf: FMap M) (mj: MJoin M) (mb: MBind M) : MBind (StateT M) :=
+  (let sj := StateT_join M mf mj in
+   let sf := StateT_fmap M mf in
+  (fun _ _ f a => mjoin (f <$> a))).
+
+Definition StateT_ret M (mr: MRet M) : MRet (StateT M) :=
+  (fun _ v => StateFn _ _ (fun s => mret (v, s))).
+
+(* Bind and Ret instances for StateT option, using the instance keyword so that the _ <- _ ; _ notation and mret work properly *)
+Instance statet_option_bind : MBind (StateT option) :=
+  StateT_bind option option_fmap option_join option_bind.
+Instance statet_option_ret : MRet (StateT option) :=
+  StateT_ret option option_ret.
+
+Definition mfail {X: Type} : StateT option X :=
+  StateFn _ _ (fun (s: state) => None).
+
+(* Turns a normal option X into a StateT option X *)
+Definition mlift {X : Type} (err_x: option X) : StateT option X :=
+
+  StateFn _ _ (fun (s: state) => match err_x with
+                              | None => None
+                              | Some x => Some (x, s)
+                              end).
+
+Definition mget {M} {_: MRet M} : StateT M state :=
+  StateFn _ _ (fun (s: state) => mret (s, s)).
+
+Definition mput {M} {_: MRet M} (newstate: state) : StateT M () :=
+  StateFn _ _ (fun (s: state) => mret ((), newstate)).
+
+Definition mupdate {M} {_: FMap M} {_: MRet M} {_: MBind M} {_: MJoin M} (f: state -> state) : StateT M () :=
+  let _ := StateT_bind M _ _ _ in
+  s <- mget;
+  mput (f s).
+
+Fixpoint interpret (fuel: nat) (e: expr) : StateT option val :=
   match fuel with
-  | O => None
+  | O => mfail
   | S n =>
     match e with
-    | Val v => Some v
-                   
-    | Var y => None
-                
-    | Rec f y e => Some (RecV f y e)
-                       
+    | Val v => mret v
+    | Var y => mfail
+    | Rec f y e => mret (RecV f y e)
     | App e1 e2 => 
-      e1' <- interpret e1 n;
+      e1' <- interpret n e1;
         match e1' with
-        | RecV BAnon BAnon ex => interpret ex n
+        | RecV BAnon BAnon ex => interpret n ex
         | RecV BAnon (BNamed y) ex =>
-          v <- interpret e2 n;
+          v <- interpret n e2;
             let e3 := subst y v ex in
-            interpret e3 n
+            interpret n e3
         | RecV (BNamed f) BAnon ex =>
-            let e3 := subst f e1' ex in
-            interpret e3 n
+          let e3 := subst f e1' ex in
+          interpret n e3
         | RecV (BNamed f) (BNamed y) ex =>
-          v <- interpret e2 n;
+          v <- interpret n e2;
             let e3 := subst f e1' (subst y v ex) in
-            interpret e3 n
-        | _ => None
+            interpret n e3
+        | _ => mfail
         end
           
     | UnOp op e =>
-      e' <- interpret e n;
-        un_op_eval op e'
+      e' <- interpret n e;
+        mlift (un_op_eval op e')
                    
     | BinOp op e1 e2 =>
-      e1' <- interpret e1 n;
-        e2' <- interpret e2 n;
-        bin_op_eval op e1' e2'
+      e1' <- interpret n e1;
+        e2' <- interpret n e2;
+        mlift (bin_op_eval op e1' e2')
                     
     | If e0 e1 e2 =>
-      c <- interpret e0 n;
+      c <- interpret n e0;
         match c with
-        | LitV (LitBool true) => interpret e1 n
-        | LitV (LitBool false) => interpret e2 n
-        | _ => None
+        | LitV (LitBool true) => interpret n e1
+        | LitV (LitBool false) => interpret n e2
+        | _ => mfail
         end
 
     | Pair e1 e2 =>
-        a <- interpret e1 n;
-        b <- interpret e2 n;
-        Some (PairV a b)
+        a <- interpret n e1;
+        b <- interpret n e2;
+        mret (PairV a b)
             
     | Fst e =>
-      e' <- interpret e n;
+      e' <- interpret n e;
       match e' with
-      | PairV v1 v2 => Some v1
-      | _ => None
+      | PairV v1 v2 => mret v1
+      | _ => mfail
       end
 
     | Snd e =>
-      e' <- interpret e n;
+      e' <- interpret n e;
       match e' with
-      | PairV v1 v2 => Some v2
-      | _ => None
+      | PairV v1 v2 => mret v2
+      | _ => mfail
       end
       
-    | InjL e => None
-    | InjR e => None
-    | Case e0 e1 e2 => None
-    | Fork e => None
-    | Primitive0 op => None
-    | Primitive1 op e => None
-    | Primitive2 op e1 e2 => None
-    | ExternalOp op e => None
-    | CmpXchg e0 e1 e2 => None
-    | NewProph => None (* ignore *)
-    | Resolve ex e1 e2 => None
+    | InjL e =>
+      v <- interpret n e;
+      mret (InjLV v)
+
+    | InjR e =>
+      v <- interpret n e;
+      mret (InjRV v)
+
+    | Case e0 e1 e2 =>
+      v <- interpret n e0;
+      match v with
+      | InjLV v' =>
+        interpret n (App e1 (Val v'))
+      | InjRV v' =>
+        interpret n (App e2 (Val v'))
+      | _ => mfail
+      end
+
+    | Fork e => mfail
+    | Primitive0 op => mfail
+    | Primitive1 op e => mfail
+    | Primitive2 op e1 e2 => mfail
+    | ExternalOp op e => mfail
+    | CmpXchg e0 e1 e2 => mfail
+    | NewProph => mfail (* ignore *)
+    | Resolve ex e1 e2 => mfail
     end
   end.
 
@@ -127,15 +207,25 @@ Definition ifStatement: expr :=
     then #3
     else #1).
 
+Definition matchtest: val :=
+  λ: "x",
+  match: (Var "x") with
+    InjL "x1" => #3 + (Var "x1")
+  | InjR "x1" => #4 + (Var "x1")
+  end.
+
 Print literalCast.
 Print testRec.
 
 End go_lang_int.
 
 (* test Fst and Snd *)
-Eval cbv in interpret (returnTwoWrapper #3) 10.
+Compute (runStateT (interpret 10 (returnTwoWrapper #3)) inhabitant).
 
-Eval cbv in (testRec _).
-Eval cbv in interpret ConstWithArith 3.
-Eval cbv in interpret (literalCast _) 1000.
-Eval cbv in interpret (useMap _) 100.
+Compute (runStateT (interpret 10 (testRec _)) inhabitant).
+Compute (runStateT (interpret 10 ConstWithArith) inhabitant).
+Compute (runStateT (interpret 10 (literalCast _)) inhabitant).
+Compute (runStateT (interpret 10 (useMap _)) inhabitant).
+Compute (runStateT (interpret 10 (ifStatement _)) inhabitant).
+Compute (runStateT (interpret 10 (matchtest (InjL #2))) inhabitant).
+Compute (runStateT (interpret 10 (matchtest (InjR #2))) inhabitant).
